Zen.Lib/extract.sh
@@ -1,0 +1,11 @@
+﻿#!/bin/bash
+
+# records hints
+../../externals/FStar/bin/fstar.exe --prims prims.fst --record_hints Consensus.Types.fst
+../../externals/FStar/bin/fstar.exe --prims prims.fst --record_hints Consensus.Realized.fst
+
+# verification and extraction of FStar to FSharp code 
+../../externals/FStar/bin/fstar.exe --codegen FSharp --prims prims.fst --extract_module Consensus.Types --use_hints --n_cores 4 --odir fs Consensus.Types.fst
+
+
+#TODO: rest source files
